

## Homework 2 For Numeric II

$$1) t_k = a + Kh, \quad K = \overline{0, N}, \quad h = \frac{b-a}{N}$$

$$y'(t) = F(t, y(t)), \quad y(a) = y_0$$

$$Y_{k+1} = Y_k + h(1-\delta)F(t_k, Y_k) + h\delta F\left(t_k + \frac{h}{2\delta}, Y_k + \frac{h}{2\delta}F(t_k, Y_k)\right), \quad \delta \in \mathbb{R}_+$$

a) Let us define the truncation error

$$\tau_k(h, \delta) = \frac{1}{h} \left[ y(t_{k+1}) - y(t_k) - h\delta F(t_k, y(t_k)) - h\delta F\left(t_k + \frac{h}{2\delta}, y(t_k) + \frac{h}{2\delta}F(t_k, y(t_k))\right) \right]$$

We know that

$$Y_{k+1} = Y_k + h\delta F(t_k, Y_k) + h\delta F\left(t_k + \frac{h}{2\delta}, Y_k + \frac{h}{2\delta}F(t_k, Y_k)\right)$$

Applying the Taylor expansion to  $Y_{k+1} = y(t_{k+1}) = y(t_k + h)$ , we have

$$y(t_{k+1}) = y(t_k) + hy'(t_k) + \frac{h^2}{2}y''(t_k) + \frac{h^3}{6}y'''(t_k) + O(h^4).$$

We also apply Taylor expansion for function  $F$ .

$$\begin{aligned} F\left(t_k + \frac{h}{2\delta}, y(t_k) + \frac{h}{2\delta}F(t_k, y(t_k))\right) &= F(t_k, y(t_k)) + \frac{h}{2\delta} \frac{\partial F}{\partial t}(t_k, y(t_k)) \\ &\quad + \frac{h}{2\delta} \frac{\partial F}{\partial y}(t_k, y(t_k))F(t_k, y(t_k)) \\ &\quad + \frac{h^2}{8\delta^2} y'''(t_k) + O(h^3) \end{aligned}$$

By expansion of numerical solution, we obtain

$$\begin{aligned} Y_{k+1} - Y_k &= h\delta F(t_k, Y_k) + h\delta \left[ F(t_k, Y_k) + \frac{h}{2\delta} y'' + \frac{h^2}{8\delta^2} y''' \right] \\ &= 2h\delta F(t_k, y(t_k)) + \frac{h^2}{2} y''(t_k) + \frac{h^3}{8\delta} y'''(t_k) + O(h^4) \end{aligned}$$

Subtract the numerical solution from the real solution, then

$$y(t_{k+1}) - y(t_k) - (Y_{k+1} - Y_k) = h(1-2\delta)F(t_k, y(t_k)) + h^3\left(\frac{1}{6} - \frac{1}{8\delta}\right)y'''(t_k) + O(h^4)$$

For consistency,  $1-2\delta=0 \Rightarrow \delta=\frac{1}{2}$ .

The result which we obtain would be divided by  $h$  in order to find the truncation error. Then, it implies

$$\tau_k(h, \delta) = \frac{h^3\left(\frac{1}{6} - \frac{1}{8\delta}\right)y'''(t_k) + O(h^4)}{h}$$

$\tau_k(h, \delta) = h^2\left(\frac{1}{6} - \frac{1}{8\delta}\right)y'''(t_k) + O(h^3)$ , but when  $\frac{\partial F}{\partial y} \neq 0$ . Then

$$\Rightarrow \tau_k(h, \delta) = \frac{h^2}{8\delta} \left[ \left( \frac{4}{3}\delta - 1 \right) y'''(t_k) + y''(t_k) \frac{\partial F}{\partial y}(t_k, y(t_k)) \right] + O(h^3)$$

b) For  $\alpha=1$ . IVP is  $y'(t) = F(t, y(t)) = -y$ ,  $\frac{\partial F}{\partial y} = -1$ .

$$(y'(t))' = (F(t, y(t)))'$$

$$y'' = \underbrace{F_t}_{F_t=0} + F_y F = F_y F = (-1)(-y) = y$$

$$y''' = (y'')' = (y)' = y' = -y. \quad (\text{By chain rule})$$

Substituting into the equation

$$\begin{aligned} \tau_k(h, \delta) &= \frac{h^2}{8\delta} \left[ \left( \frac{4}{3}\delta - 1 \right) (-y) + y(-1) \right] + O(h^3) \\ &= \frac{h^2}{8\delta} \left[ -\left( \frac{4}{3}\delta y \right) \right] + O(h^3) = -\frac{h^2}{6} y + O(h^3) \end{aligned}$$

$$\frac{\tau_k(h, \delta)}{h} = \frac{-h}{6} y + O(h^2)$$



For  $\alpha \geq 2$ ,  $y' = -y^\alpha$ ,  $\frac{\partial f}{\partial y} = -\alpha y^{\alpha-1}$ .

$$y' = -y^\alpha$$

$$y'' = f_y f = (-\alpha y^{\alpha-1})(-y^\alpha) = \alpha y^{2\alpha-1}$$

$$y''' = (y'')' = (\alpha y^{2\alpha-1})' = \alpha(2\alpha-1)y^{2\alpha-2} y' = \alpha(2\alpha-1)y^{2\alpha-2}(-y^\alpha)$$

$$y'' f_y = (\alpha y^{2\alpha-1})(-\alpha y^{\alpha-1}) = -\alpha^2 y^{3\alpha-2} = -\alpha(2\alpha-1)y^{3\alpha-2}$$

In order to vanish the part of  $h^2$ , we apply

$$\left(\frac{4}{3}\delta - 1\right) y''' + y'' f_y = 0$$

$$\Rightarrow \left(\frac{4}{3}\delta - 1\right)(-\alpha(2\alpha-1)y^{3\alpha-2}) + (-\alpha^2 y^{3\alpha-2}) = 0$$

$$-\left(\frac{4}{3}\delta - 1\right)\alpha(2\alpha-1) - \alpha^2 = 0$$

$$-\left(\frac{4}{3}\delta - 1\right)(2\alpha-1) - \alpha = 0 \Rightarrow -\left(\frac{4}{3}\delta - 1\right)(2\alpha-1) = \alpha$$

$$\Rightarrow \frac{4}{3}\delta - 1 = \frac{-\alpha}{2\alpha-1} \Rightarrow \frac{4}{3}\delta = 1 - \frac{\alpha}{2\alpha-1}$$

$$\Rightarrow \frac{4}{3}\delta = \frac{\alpha-1}{2\alpha-1}$$

$$\Rightarrow \delta = \frac{3(\alpha-1)}{4(2\alpha-1)}, \text{ since } \alpha \geq 2, \delta > 0.$$

So, we find  $\delta_0 \in \mathbb{R}^+$ .

Thus, the truncation error would be the term of  $O(h^3)$ .

$$2) y'(t) = f(t, y(t)), \quad a \leq t \leq b$$

$$y(a) = y_0$$

$$\|\Phi(t, y_1, h) - \Phi(t, y_2, h)\| \leq L \|y_1 - y_2\|, \quad y_1, y_2 \in \mathbb{R}^n$$

$$\langle y_1 - y_2, \Phi(t, y_1, h) - \Phi(t, y_2, h) \rangle \leq \Theta \|y_1 - y_2\|^2 \text{ for } \Theta \in \mathbb{R}.$$

Proof:

Let us define the global error  $e_k = y(t_k) - Y_k$ . Then, by the one-step method, we have

$$e_{k+1} = e_k + h_k [\Phi(t_k, y(t_k), h_k) - \Phi(t_k, Y_k, h_k)] + h_k \tau(t_k, h_k).$$

Take the inner product of  $e_{k+1}$ , then

$$\begin{aligned} \|e_{k+1}\|^2 &= \|e_k\|^2 + 2h_k \langle e_k, \Phi(t_k, y(t_k), h_k) - \Phi(t_k, Y_k, h_k) \rangle \\ &\quad + h_k^2 \|\Phi(t_k, y(t_k), h_k) - \Phi(t_k, Y_k, h_k)\|^2 \\ &\quad + \text{error terms from } \tau \end{aligned}$$

By the given inequalities, it means

$$\begin{aligned} \langle e_k, \Phi(t_k, y(t_k), h_k) - \Phi(t_k, Y_k, h_k) \rangle &\leq \Theta \|e_k\|^2 \\ \|\Phi(t_k, y(t_k), h_k) - \Phi(t_k, Y_k, h_k)\| &\leq L \|e_k\|. \end{aligned}$$

So,

$$\begin{aligned} \|e_{k+1}\|^2 &\leq (1 + 2h_k \Theta + h_k^2 L^2) \|e_k\|^2 + 2h_k \langle e_k, \tau(t_k, h_k) \rangle \\ &\quad + h_k^2 \|\tau(t_k, h_k)\|^2 \\ &\rightarrow \leq (1 + 2h_k \Theta + h_k^2 L^2) \|e_k\|^2 + h_k^2 (1 + L^2) \|\tau(t_k, h_k)\|^2. \end{aligned}$$

Cauchy-Schwarz

If we take the square root, then

$$\|e_{k+1}\| \leq \sqrt{1 + 2h_k \Theta + h_k^2 L^2} \|e_k\| + h_k \|\tau(t_k, h_k)\|.$$



Denote  $\sqrt{1+2h_k\theta+h_k^2L^2} \leq e^{\left(\frac{1}{2}(2h_k\theta+h_k^2L^2)\right)}$   
 $= e^{(h_k\theta+\frac{1}{2}h_k^2L^2)}$

Hence,  $\|e_{k+1}\| \leq e^{(h_k\theta+\frac{1}{2}h_k^2L^2)} \|e_k\| + h_k \|\tau(t_k, h_k)\|$ .

Now, let us apply the Gronwall, then

$$\begin{aligned} \|e_k\| &\leq \sum_{j=0}^{k-1} (h_j \|\tau(t_j, h_j)\|) \prod_{m=j+1}^{k-1} e^{(h_m\theta+\frac{1}{2}h_m^2L^2)} \\ &= \sum_{j=0}^{k-1} h_j \|\tau(t_j, h_j)\| e^{\left(\sum_{m=j+1}^{k-1} (h_m\theta+\frac{1}{2}h_m^2L^2)\right)} \end{aligned}$$

In order to bound the sums, we use

$$\sum_{m=j+1}^{k-1} h_m \leq t_k - a, \quad \sum_{m=j+1}^{k-1} h_m^2 \leq h \sum_{m=j+1}^{k-1} h_m \leq h(t_k - a)$$

Then,  $\sum_{m=j+1}^{k-1} (h_m\theta+\frac{1}{2}h_m^2L^2) \leq \theta(t_k - a) + \frac{1}{2}L^2h(t_k - a)$ .

Thus,  $\|e_k\| \leq e^{(\theta(t_k - a) + \frac{1}{2}L^2h(t_k - a))} \sum_{j=0}^{k-1} h_j \|\tau(t_j, h_j)\|$ .

Therefore,

$$\|y(t_k) - y_k\| \leq e^{(\theta(t_k - a) + \frac{1}{2}L^2h(t_k - a))} \sum_{j=0}^{k-1} h_j \|\tau(t_j, h_j)\|$$

where,  $k = 1, \dots, N$  and for  $h = \max_K h_k$ .

□